\section*{3.1 Multiplying Out and Factoring Expressions}
Following theorems are useful in factoring and multiplying out (Very Useful for Bolean Expression Manipulation):
\begin{align}
    X(Y + Z) = XY + XZ\\
    (X + Y)(X + Z) = X + YZ \label{eq:2}\\
    (X+Y)(X^\prime+Z)=XZ+X^\prime Y \label{eq:3}
\end{align}
\subsection*{Proving}
Theorem \ref{eq:2}:
\begin{align*}
    (X + Y)(X + Z)&=X+XY+XZ+YZ\\
    &=X(1+Y+Z)+YZ\\
    &=X+YZ
\end{align*}
Theorem \ref{eq:3}:
\begin{align*}
    (X+Y)(X^\prime+Z)=0+XZ+YX^\prime + YZ\\
\end{align*}
Putting X=0
\begin{align*}
    X&=0\\
    Y&=Y+YZ\\
    Y&=Y
\end{align*}
Putting X=1
\begin{align*}
    X&=1\\
    Z&=Z+YZ\\
    Z&=Z
\end{align*}
Hence Proved\\
\subsection*{Examples}
\begin{enumerate}
    \item $(Q + AB^\prime)(C^\prime D + Q^\prime)$\\
    Use \ref{eq:3}\\
    $= QAB^\prime+Q^\prime C^\prime D$
    \item $[(A + B + C^\prime)(A + B + D)](A + B + E)(A + D^\prime + E)(A^\prime + C)$\\
    Using \ref{eq:2}\\
    $=[(A + B + C^\prime D)(A + B + E)][(A + D^\prime + E)(A^\prime + C)]$\\
    Using \ref{eq:2} and \ref{eq:3}\\
    $=(A+B+C^\prime DE)(AC+A^\prime(D^\prime+E))$\\
    $=[AC+ABC]+A^\prime BD^\prime +A^\prime BE+ A^\prime C^\prime DE$\\
    $=AC+A^\prime BD^\prime +A^\prime BE+ A^\prime C^\prime DE$    
\end{enumerate}
